bvpProps evaluate_locals

compiler1/semantics/bvpPropsScript.sml
@@ -3,6 +3,10 @@ local open sourcePropsTheory in end;
 
 val _ = new_theory"bvpProps";
 
+val with_same_locals = store_thm("with_same_locals",
+  ``(s with locals := s.locals) = s``,
+  fs [state_component_equality]);
+
 val EVERY_get_vars = store_thm("EVERY_get_vars",
   ``!args s1 s2.
       EVERY (\a. lookup a s1.locals = lookup a s2.locals) args ==>
@@ -20,18 +24,18 @@ val get_vars_IMP_domain = store_thm("get_vars_IMP_domain",
 val get_vars_with_stack = prove(
   ``!args s. (s.locals = t.locals) ==>
              (get_vars args s = get_vars args t)``,
-  Induct \\ fs [get_vars_def,get_var_def])
+  Induct \\ fs [get_vars_def,get_var_def]);
 
 val get_vars_with_stack_rwt = prove(
   ``(get_vars args (s with stack := xs) = get_vars args s) /\
     (get_vars args (s with <| locals := l ; stack := xs |>) =
      get_vars args (s with <| locals := l |>))``,
   REPEAT STRIP_TAC
-  \\ MATCH_MP_TAC get_vars_with_stack \\ fs [])
+  \\ MATCH_MP_TAC get_vars_with_stack \\ fs []);
 
 val cut_state_opt_with_stack = Q.prove(
   `cut_state_opt x (y with stack := z) = OPTION_MAP (λs. s with stack := z) (cut_state_opt x y)`,
-  EVAL_TAC >> every_case_tac >> simp[])
+  EVAL_TAC >> every_case_tac >> simp[]);
 
 val consume_space_with_stack = Q.prove(
   `consume_space x (y with stack := z) = OPTION_MAP (λs. s with stack := z) (consume_space x y)`,
@@ -49,7 +53,7 @@ val do_app_with_stack = Q.prove(
 val do_app_with_locals = Q.prove(
   `do_app op vs (s with locals := z) = map_result (λ(x,y). (x,y with locals := z)) I (do_app op vs s)`,
   rw[do_app_def,do_space_def,bvi_to_bvp_def,bvp_to_bvi_def] >>
-  every_case_tac >> fs[consume_space_with_locals] >> rw[] >> fs[])
+  every_case_tac >> fs[consume_space_with_locals] >> rw[] >> fs[]);
 
 val do_app_err = Q.store_thm("do_app_err",
   `do_app op vs s = Rerr e ⇒
@@ -70,6 +74,18 @@ val do_app_const = Q.store_thm("do_app_const",
   fs[bviSemTheory.do_app_def] >>
   every_case_tac >> fs[] >> rpt var_eq_tac >>
   fs[consume_space_def] >> var_eq_tac >> simp[])
+
+val do_app_locals = store_thm("do_app_locals",
+  ``(do_app op x s = Rval (q,r)) ==>
+    (do_app op x (s with locals := extra) =
+       Rval (q,r with locals := extra))``,
+  fs [do_app_def,do_space_def,consume_space_def,bvp_to_bvi_def]
+  \\ every_case_tac >> fs[] \\ SRW_TAC [] []
+  \\ fs [bvi_to_bvp_def,state_component_equality]);
+
+val Seq_Skip = store_thm("Seq_Skip",
+  ``evaluate (Seq c Skip,s) = evaluate (c,s)``,
+  fs [evaluate_def] \\ Cases_on `evaluate (c,s)` \\ fs [LET_DEF] \\ SRW_TAC [] []);
 
 val evaluate_stack_swap = Q.store_thm("evaluate_stack_swap",
   `!c s.
@@ -383,5 +399,157 @@ val evaluate_locals_LN = store_thm("evaluate_locals_LN",
       (evaluate (c,s) = (res,t)) /\ res <> NONE /\ res <> SOME (Rerr(Rabort Rtype_error)) ==>
       (t.locals = LN) \/ ?t. res = SOME (Rerr(Rraise t))``,
   REPEAT STRIP_TAC \\ MP_TAC (SPEC_ALL evaluate_locals_LN_lemma) \\ fs []);
+
+val locals_ok_def = Define `
+  locals_ok l1 l2 =
+    !v x. (sptree$lookup v l1 = SOME x) ==> (sptree$lookup v l2 = SOME x)`;
+
+val locals_ok_IMP = prove(
+  ``locals_ok l1 l2 ==> domain l1 SUBSET domain l2``,
+  fs [locals_ok_def,SUBSET_DEF,domain_lookup] \\ METIS_TAC []);
+
+val locals_ok_refl = store_thm("locals_ok_refl",
+  ``!l. locals_ok l l``,
+  fs [locals_ok_def]);
+
+val locals_ok_cut_env = store_thm("locals_ok_cut_env",
+  ``locals_ok l1 l2 /\
+    (cut_env names l1 = SOME x) ==>
+    (cut_env names l2 = SOME x)``,
+  fs [cut_env_def] \\ SRW_TAC [] []
+  THEN1 (IMP_RES_TAC locals_ok_IMP \\ IMP_RES_TAC SUBSET_TRANS)
+  \\ fs [lookup_inter_alt] \\ SRW_TAC [] []
+  \\ fs [locals_ok_def,domain_lookup,SUBSET_DEF,PULL_EXISTS]
+  \\ fs [oneTheory.one] \\ RES_TAC \\ RES_TAC \\ fs []);
+
+val locals_ok_get_var = store_thm("locals_ok_get_var",
+  ``locals_ok s.locals l /\
+    (get_var x s = SOME w) ==>
+    (get_var x (s with locals := l) = SOME w)``,
+  fs [locals_ok_def,get_var_def]);
+
+val locals_ok_get_vars = store_thm("locals_ok_get_vars",
+  ``!x w.
+      locals_ok s.locals l /\
+      (get_vars x s = SOME w) ==>
+      (get_vars x (s with locals := l) = SOME w)``,
+  Induct \\ fs [get_vars_def] \\ REPEAT STRIP_TAC
+  \\ Cases_on `get_var h s` \\ fs []
+  \\ Cases_on `get_vars x s` \\ fs []
+  \\ IMP_RES_TAC locals_ok_get_var \\ fs []);
+
+val bvp_to_bvi_with_locals = Q.store_thm("bvp_to_bvi_with_locals",
+  `bvp_to_bvi (s with locals := l) = bvp_to_bvi s`,
+  EVAL_TAC)
+
+val bvi_to_bvp_with_locals = Q.store_thm("bvi_to_bvp_with_locals",
+  `bvi_to_bvp t (s with locals := l) = (bvi_to_bvp t s) with locals := l`,
+  EVAL_TAC)
+
+val evaluate_locals = store_thm("evaluate_locals",
+  ``!c s res s2 vars l.
+      res <> SOME (Rerr(Rabort Rtype_error)) /\ (evaluate (c,s) = (res,s2)) /\
+      locals_ok s.locals l ==>
+      ?w. (evaluate (c, s with locals := l) =
+             (res,if res = NONE then s2 with locals := w
+                                else s2)) /\
+          locals_ok s2.locals w``,
+  recInduct evaluate_ind \\ REPEAT STRIP_TAC \\ fs [evaluate_def]
+  THEN1 (* Skip *) (METIS_TAC [])
+  THEN1 (* Move *)
+   (Cases_on `get_var src s` \\ fs [] \\ SRW_TAC [] []
+    \\ IMP_RES_TAC locals_ok_get_var \\ fs []
+    \\ fs [get_var_def,lookup_union,set_var_def,locals_ok_def]
+    \\ Q.EXISTS_TAC `insert dest x l` \\ fs [lookup_insert]
+    \\ METIS_TAC [])
+  THEN1 (* Assign *)
+   (Cases_on `names_opt` \\ fs []
+    \\ Cases_on `op_space_reset op` \\ fs [cut_state_opt_def] THEN1
+     (Cases_on `get_vars args s` \\ fs [cut_state_opt_def]
+      \\ IMP_RES_TAC locals_ok_get_vars \\ fs []
+      \\ reverse(Cases_on `do_app op x s`) \\ fs [] >- (
+           imp_res_tac do_app_err >> fs[] >>
+           Cases_on`a`>>fs[] >> rw[] >>
+           fs[do_app_def,do_space_def,bvp_to_bvi_with_locals,
+              bvi_to_bvp_with_locals,
+              bvi_to_bvpTheory.op_space_req_def,
+              bvi_to_bvpTheory.op_space_reset_def] >>
+           BasicProvers.CASE_TAC >> fs[] >- (
+             Cases_on`a`>>fs[] ) >>
+           simp[call_env_def,locals_ok_def,lookup_fromList])
+      \\ Cases_on `a` \\ fs [] \\ SRW_TAC [] []
+      \\ IMP_RES_TAC do_app_locals \\ fs [set_var_def]
+      \\ Q.EXISTS_TAC `insert dest q l`
+      \\ fs [set_var_def,locals_ok_def,lookup_insert]
+      \\ METIS_TAC [do_app_const])
+    \\ fs [cut_state_def]
+    \\ Cases_on `cut_env x s.locals` \\ fs []
+    \\ IMP_RES_TAC locals_ok_cut_env \\ fs []
+    \\ Q.EXISTS_TAC `s2.locals` \\ fs [locals_ok_def]
+    \\ SRW_TAC [] [state_component_equality])
+  THEN1 (* Tick *)
+   (Cases_on `s.clock = 0` \\ fs [] \\ SRW_TAC [] []
+    \\ fs [locals_ok_def,call_env_def,EVAL ``fromList []``,lookup_def,
+           dec_clock_def] \\ METIS_TAC [])
+  THEN1 (* MakeSpace *)
+   (Cases_on `cut_env names s.locals` \\ fs []
+    \\ IMP_RES_TAC locals_ok_cut_env
+    \\ fs [LET_DEF,add_space_def,state_component_equality,locals_ok_def])
+  THEN1 (* Raise *)
+   (Cases_on `get_var n s` \\ fs [] \\ SRW_TAC [] []
+    \\ `jump_exc (s with locals := l) = jump_exc s` by
+         fs [jump_exc_def] \\ Cases_on `jump_exc s` \\ fs []
+    \\ `get_var n (s with locals := l) = SOME x` by
+         fs [locals_ok_def,get_var_def] \\ fs []
+    \\ srw_tac [] [] \\ Q.EXISTS_TAC `s2.locals`
+    \\ fs [locals_ok_def])
+  THEN1 (* Return *)
+   (Cases_on `get_var n s` \\ fs [] \\ SRW_TAC [] []
+    \\ `get_var n (s with locals := l) = SOME x` by
+         fs [locals_ok_def,get_var_def] \\ fs []
+    \\ srw_tac [] [call_env_def]
+    \\ simp[locals_ok_def,lookup_fromList])
+  THEN1 (* Seq *)
+   (Cases_on `evaluate (c1,s)` \\ fs [LET_DEF]
+    \\ Cases_on `q = SOME (Rerr(Rabort Rtype_error))` \\ fs []
+    \\ FIRST_X_ASSUM (MP_TAC o Q.SPEC `l`) \\ fs []
+    \\ REPEAT STRIP_TAC \\ fs []
+    \\ Cases_on `q` \\ fs [] \\ SRW_TAC [] [] \\ METIS_TAC [])
+  THEN1 (* If *)
+   (Cases_on `evaluate (g,s)` \\ fs []
+    \\ REVERSE (Cases_on `q`) \\ fs []
+    \\ SRW_TAC [] [] \\ fs []
+    \\ FIRST_X_ASSUM (STRIP_ASSUME_TAC o Q.SPEC `l`) \\ fs []
+    \\ REV_FULL_SIMP_TAC (srw_ss()) []
+    THEN1 METIS_TAC [locals_ok_def]
+    \\ Cases_on `get_var n r` \\ fs []
+    \\ IMP_RES_TAC locals_ok_get_var \\ fs []
+    \\ Cases_on `x = Boolv T` \\ fs []
+    \\ Cases_on `x = Boolv F` \\ fs [])
+  THEN1 (* Call *)
+   (Cases_on `s.clock = 0` \\ fs [] \\ SRW_TAC [] []
+    THEN1 (fs [locals_ok_def,call_env_def,EVAL ``fromList []``,lookup_def,
+             dec_clock_def] \\ METIS_TAC [])
+    \\ Cases_on `get_vars args s` \\ fs []
+    \\ IMP_RES_TAC locals_ok_get_vars \\ fs []
+    \\ Cases_on `find_code dest x s.code` \\ fs []
+    \\ Cases_on `x'` \\ fs []
+    \\ Cases_on `ret` \\ fs [] THEN1
+     (Cases_on `handler` \\ fs []
+      \\ `call_env q (dec_clock (s with locals := l)) =
+          call_env q (dec_clock s)` by
+         fs [state_component_equality,dec_clock_def,call_env_def] \\ fs []
+      \\ Q.EXISTS_TAC `s2.locals` \\ fs [locals_ok_refl]
+      \\ SRW_TAC [] [state_component_equality])
+    \\ Cases_on `x'` \\ fs []
+    \\ Cases_on `cut_env r' s.locals` \\ fs []
+    \\ IMP_RES_TAC locals_ok_cut_env \\ fs []
+    \\ `call_env q (push_env x' (IS_SOME handler)
+          (dec_clock (s with locals := l))) =
+        call_env q (push_env x' (IS_SOME handler)
+          (dec_clock s))` by ALL_TAC THEN1
+     (Cases_on `handler`
+      \\ fs [state_component_equality,dec_clock_def,call_env_def,push_env_def])
+    \\ fs [] \\ METIS_TAC [locals_ok_refl,with_same_locals]));
 
 val _ = export_theory();
